{
 "cells": [
  {
   "cell_type": "markdown",
   "metadata": {},
   "source": [
    "HW Liwei\n",
    "\n",
    "$E = \\sum_{i,M}^{}P_i(M)E_i(M)$ <br /><br /> Due to total derivative<br /><br />\n",
    "$dE = \\sum_{i,M}^{}\\frac{\\partial P_i(M)E_i(M)}{\\partial P_i(M)}dP_i(M) + \\sum_{i,M}^{}\\frac{\\partial P_i(M)E_i(M)}{\\partial E_i(M)}dE_i(M)$<br /><br />$=\\sum_{i,M}^{}E_i(M)dP_i(M) + \\sum_{i,M}^{}P_i(M)dE_i(M)$ <br /><br />Similarly, from $N=\\sum_{i,M}MP_i(M),$<br /><br />$dN=\\sum_{i,M}^{}\\frac{\\partial MP_i(M)}{\\partial P_i(M)}dP_i(M) + \\sum_{i,M}^{}\\frac{\\partial MP_i(M)}{\\partial M}dM$<br /><br />$=\\sum_{i,M}^{}MdP_i(M) + \\sum_{i,M}^{}P_i(M)dM$<br /><br />$=\\sum_{i,M}^{}MdP_i(M)$   ($dM = 0$ because each M is treated as a constant)"
   ]
  },
  {
   "cell_type": "markdown",
   "metadata": {},
   "source": [
    "HW Liwei\n",
    "\n",
    "What are the values of the probabilities for which we obtain a maximum entropy?\n",
    "\n",
    "$$S = -k\\sum_{t}P_tlnP_t$$\n",
    "\n",
    "#### Prove_1: Lagrange multiplier\n",
    "\n",
    "$S = -k\\sum_{t}P_tlnP_t$<br />\n",
    "\n",
    "Constraints: $g = \\sum_{t}P_t = 1$<br />\n",
    "\n",
    "$\\frac{\\partial}{\\partial P_t}(S + \\lambda(g - 1)) = 0$ <br/>\n",
    "\n",
    "Then,\n",
    "\n",
    "$\\frac{\\partial}{\\partial P_t}(-k\\sum_{t}P_tlnP_t + \\lambda(g - 1)) = 0$ <br/>\n",
    "\n",
    "After calculating the first derivative for each $P_t$, we get\n",
    "\n",
    "$-k(1 + lnP_t) + \\lambda = 0$<br />\n",
    "\n",
    "which means $S$ is the maximum when all $P_t$ are equal, due to the constraint $g = \\sum_{t}P_t = 1$<br />\n",
    "\n",
    "$P_t = \\frac{1}{n}$  ($n$ is the number of $P_t$)\n",
    "\n",
    "#### Prove_2:  Use inequation $lnx <= x-1$\n",
    "\n",
    "Assumption: $S_{max} = lnM$, then <br />\n",
    "\n",
    "$k\\sum_{t}P_tln\\frac{1}{P_t} - S_{max} <= 0$<br />\n",
    "\n",
    "$k\\sum_{t}P_tln\\frac{1}{P_t} - k\\sum_{t}P_t\\frac{1}{k}lnM <= 0$   (because $\\sum_{t}P_t = 1$)\n",
    "\n",
    "$k\\sum_{t}P_t(ln\\frac{1}{P_t}-\\frac{1}{k}lnM) <= 0$\n",
    "\n",
    "$k\\sum_{t}P_t(ln\\frac{1}{P_t}-\\frac{1}{k}lnM) <= k\\sum_{t}P_t(\\frac{1}{P_tM^\\frac{1}{k}}-1)$\n",
    "\n",
    "$k\\sum_{t}P_t(ln\\frac{1}{P_t}-\\frac{1}{k}lnM) = k\\sum_{t}P_t(\\frac{1}{P_tM^\\frac{1}{k}}-1)$ if and only if left and right side equal to zero, and now $S = -k\\sum_{t}P_tlnP_t$ become $S_{max}$.\n",
    "\n",
    "From the left side, $k\\sum_{t}P_t(ln\\frac{1}{P_t}-\\frac{1}{k}lnM) = 0$\n",
    "\n",
    "$\\frac{1}{P_tM^\\frac{1}{k}} = 1$\n",
    "\n",
    "we get $P_t = M^{-\\frac{1}{k}}$\n",
    "\n",
    "From the right side, $k\\sum_{t}P_t(\\frac{1}{P_tM^\\frac{1}{k}}-1) = 0$\n",
    "\n",
    "we get $N^k = M$\n",
    "\n",
    "Thus, $P_t = \\frac{1}{n}$   ($n$ is the number of $P_t$)"
   ]
  },
  {
   "cell_type": "markdown",
   "metadata": {},
   "source": [
    "$N =$ _O(N)_ and $\\mu$ = _O(kT)_ which can be ignored considering the order of $N$, so $(\\frac{dN}{d\\mu})_{V,T}$ = _O(N)_"
   ]
  },
  {
   "cell_type": "markdown",
   "metadata": {},
   "source": [
    "### Prove $\\frac{\\partial <N_i>}{\\partial T} = \\frac{<N_i>(\\epsilon_i - <\\epsilon>)}{kT^2}$\n",
    "\n",
    "$\\eta_i = \\frac{e^{-\\epsilon_i/kT}}{q} \\space $ (1)\n",
    "\n",
    "$<N_i> = N\\eta_i \\space $ (2)\n",
    "\n",
    "$q = \\sum_i e^{-\\epsilon_i/kT} \\space$ (3)\n",
    "\n",
    "$<\\epsilon> = \\frac{1}{q}\\sum_i\\epsilon_ie^{-\\epsilon_i/kT} \\space$ (4)\n",
    "\n",
    "$\\frac{\\partial <N_i>}{\\partial T} = N\\frac{\\partial\\frac {e^{-\\epsilon_i/kT}}{q}}{\\partial T}$\n",
    "\n",
    "$ = N\\frac{\\frac{\\epsilon_i}{kT^2}e^{\\frac{-\\epsilon_i}{kT}}q - \\frac{\\partial q}{\\partial T}e^{\\frac{-\\epsilon_i}{kT}}}{q^2}$\n",
    "\n",
    "$ = N\\frac{\\frac{\\epsilon_i}{kT^2}e^{\\frac{-\\epsilon_i}{kT}}q - \\frac{1}{kT^2}e^{\\frac{-\\epsilon_i}{kT}}\\sum\\epsilon_ie^{\\frac{-\\epsilon_i}{kT}}}{q^2}$\n",
    "\n",
    "$ = N\\frac{e^{\\frac{-\\epsilon_i}{kT}}}{q}\\frac{\\epsilon_i - <\\epsilon>}{kT^2} = \\frac{<N_i>(\\epsilon_i - <\\epsilon>)}{kT^2} \\space$ from (1),(2),(3) and (4)"
   ]
  },
  {
   "cell_type": "markdown",
   "metadata": {},
   "source": [
    "#### Possible degeneracy of $\\epsilon_{l_xl_yl_z} = \\frac{h^2(l_x^2 + l_y^2 + l_z^2)}{8mL^2}$  $(l_x, l_y, l_z = 1,2,3,...)$\n",
    "\n",
    "Three conditions:\n",
    "1. no degeneracy when $l_x = l_y = l_z$\n",
    "2. 3 degeneracies when two out of $l_x, l_y, l_z$ are the same and the other one is different. could be \n",
    "   $l_x = l_y \\ne l_z$;$\\space l_x = l_z \\ne l_y$; $\\space l_y = l_z \\ne l_x$\n",
    "3. 6 degeneracies when $l_x \\ne l_z \\ne l_y$ like (1,2,3);(1,3,2);(2,1,3);(2,3,1);(3,1,2);(3,2,1)\n",
    "\n",
    "2-d Geometric proof:\n",
    "\n",
    "Degeneracy: $l_x^2 + l_y^2 = l_m^2 + l_n^2\\space$, which means the distance of two points in 2-d cartesian coordinates with positive integer points $(l_x, l_y)$ and $(l_m, l_n)$ to origin $(0,0)$, if $l_x = l_y$, $l_x = l_y = l_m = l_n$ because the distance of any other points to $(0,0)$ are longer or shorter; if $l_x \\ne l_y$, there are two degeneracies, which two points are symmetric in terms of the line $y = x$. This can be expanded to 3-d coordinates.\n",
    "\n",
    "#### Quantum number of electron in the cube \n",
    "\n",
    "Electrons in a cube only have spin quantum number which obeys Fermiâ€“Dirac statistics.\n",
    "\n",
    "#### __$\\lambda = O(\\frac{h}{mv})$__\n",
    "\n",
    "In the cube, each particle only has kinetic energy, so\n",
    "\n",
    "$\\lambda = O(\\frac{h}{(2\\pi m*\\frac{1}{2}mv^2)^{1/2}} ) = O(\\frac{h}{mv})$\n"
   ]
  },
  {
   "cell_type": "markdown",
   "metadata": {},
   "source": [
    "#### Experiments are done under T $\\rightarrow$ 0 when ground state is non-degenerate\n",
    "1. One particle in the box and measure the energy $E_1$\n",
    "\n",
    "   Ten particles in the box and measure the energy $E_2$\n",
    "   \n",
    "   If $E_2 = 10E_1$, then the particles are bosons, otherwise they are fermions.\n",
    "   \n",
    "\n",
    "2. It is impossible to attain absolute zero of temperature."
   ]
  },
  {
   "cell_type": "markdown",
   "metadata": {},
   "source": [
    "#### Fermi-Dirac Micro-canonical treatment\n",
    "\n",
    "$L\\left(m_{i}, \\alpha, \\beta\\right)=\\ln W-\\alpha\\left(\\sum_{i} m_{i}-N\\right)-\\beta\\left(\\sum_{i} m_{i} \\varepsilon_{i}-E\\right)$\n",
    "\n",
    "$ = \\sum_{i}\\ln W_i-\\alpha\\left(\\sum_{i} m_{i}-N\\right)-\\beta\\left(\\sum_{i} m_{i} \\varepsilon_{i}-E\\right)$\n",
    "\n",
    "$ = \\ln W_i^* -\\alpha\\left(\\sum_{i} m_{i}-N\\right)-\\beta\\left(\\sum_{i} m_{i} \\varepsilon_{i}-E\\right)$\n",
    "\n",
    "$ = \\ln g_i!-\\ln (g_i - m_i)! -\\ln(m_i)!-\\alpha\\left(\\sum_{i} m_{i}-N\\right)-\\beta\\left(\\sum_{i} m_{i} \\varepsilon_{i}-E\\right)$\n",
    "\n",
    "$ = -[(g_i - m_i)\\ln(g_i - m_i) - (g_i - m_i)] - (m_i\\ln m_i - m_i) - \\alpha\\left(\\sum_{i} m_{i}-N\\right)-\\beta\\left(\\sum_{i} m_{i} \\varepsilon_{i}-E\\right)$\n",
    "\n",
    "$\\frac{\\partial L\\left(m_{i}, \\alpha, \\beta\\right)}{\\partial m_i} = \\ln(g_i - m_i) -\\ln m_i -\\alpha - \\beta \\varepsilon_{i} = 0$\n",
    "\n",
    "$\\ln\\frac{g_i-m_i}{m_i} = \\alpha +\\beta \\varepsilon_{i}$\n",
    "\n",
    "$\\frac{g_i}{m_i} -1 = e^{(\\alpha+\\beta\\varepsilon_{i})}$\n",
    "\n",
    "$<n_i> = \\frac{m_i}{g_i} = \\frac{1}{1+e^{-(\\alpha+\\beta\\varepsilon_{i})}}$\n",
    "\n",
    "Considering microcanonical ensemble is a degenerate grandcanonical ensemble, after comparing with result of grandcanonical ensemble, \n",
    "\n",
    "$\\alpha = -\\frac{\\mu}{kT}$, $\\beta = \\frac{1}{kT}$\n",
    "\n",
    "so \n",
    "\n",
    "$<n_i> = \\frac{1}{1+e^{\\frac{\\varepsilon_{i}-\\mu}{k T}}}$\n"
   ]
  },
  {
   "cell_type": "markdown",
   "metadata": {},
   "source": [
    "#### Bose-Einstein Micro-canonical treatment\n",
    "\n",
    "The only difference with the Fermi-Dirac Micro-canonical treatment is the form of $W_i$.\n",
    "\n",
    "By substituting $W_i = \\frac{(m_i+g_i)!}{g_i!m_i!}$ into above treatment\n",
    "\n",
    "we get\n",
    "\n",
    "$\\ln\\frac{g_i+m_i}{m_i} = \\alpha +\\beta \\varepsilon_{i}$\n",
    "\n",
    "so \n",
    "\n",
    "$<n_i> = \\frac{1}{e^{\\frac{\\varepsilon_{i}-\\mu}{k T}}-1}$"
   ]
  },
  {
   "cell_type": "markdown",
   "metadata": {},
   "source": [
    "$U(x)=\\sum_{i=1}^{N}\\left[u\\left(a+x_{i+1}-x_{i}\\right)+u\\left(2 a+x_{i+2}-x_{i}\\right)\\right] \\space (1)$\n",
    "\n",
    "__After \"uncouple\",__\n",
    "\n",
    "$\\begin{aligned} u(a+\\delta) &=u(a)+u^{\\prime}(a) \\delta+\\frac{1}{2} u^{\\prime \\prime}(a) \\delta^{2}+\\cdots \\space (2)\\\\ u(2 a+\\eta) &=u(2 a)+u^{\\prime}(2 a) \\eta+\\frac{1}{2} u^{\\prime \\prime}(2 a) \\eta^{2}+\\cdots \\space (3)\\end{aligned}$\n",
    "\n",
    "__where $\\delta = x_{i+1} - x_i; \\eta = x_(i+2) - x_i$;__\n",
    "\n",
    "$u^\\prime(a) = 0; u^\\prime(2a) = 0 \\space$__because $u(x)$ has minimum at $x_i = 0$ for all i__\n",
    "\n",
    "__So, after substituting (2) and (3) into (1), all $u^\\prime(a)\\delta = 0; u^\\prime(2a)\\eta = 0.\\space$__"
   ]
  },
  {
   "cell_type": "markdown",
   "metadata": {},
   "source": [
    "#### Thermodynamics of Quantum states\n",
    "\n",
    "##### Canonical Ensemble\n",
    "\n",
    "$\\frac{\\partial}{\\partial \\omega_{n}}\\{-k T r(\\rho \\ln \\rho)-\\beta[\\operatorname{Tr}(\\rho H)-E]-\\alpha[\\operatorname{Tr}(\\rho)-1]\\}=0 \\space $   (1)\n",
    "\n",
    "$\\operatorname{Tr}(\\rho \\ln \\rho)=\\sum_{n} \\omega_{n} \\ln \\omega_{n} \\space$  (2)\n",
    "\n",
    "$\\operatorname{Tr}(H \\rho)=\\langle\\psi|H| \\psi\\rangle=\\sum_{n} \\omega_{n}\\left\\langle\\psi_{n}|H| \\psi_{n}\\right\\rangle \\space$  (3)\n",
    "\n",
    "$\\operatorname{Tr}(\\rho)=\\sum_{n} \\omega_{n} \\space$  (4)\n",
    "\n",
    "For $\\omega_n$, which would lead largest Von Neumann entropy, by substituting (2),(3),(4) into (1), we get\n",
    "\n",
    "$-k\\ln\\omega_n - 1 - \\beta E_n - \\alpha = 0 \\space$  (5) \n",
    "\n",
    "$\\omega_n = e^{-\\frac{(\\beta E_n + \\alpha + 1)}{k}} \\space$  (6)\n",
    "\n",
    "$\\sum_{n} \\omega_n = 1 \\space$ (7)\n",
    "\n",
    "then,\n",
    "\n",
    "$\\omega_n = \\frac{e^{-\\beta E_n}}{\\sum_{e^{-\\beta E_n}}}$\n",
    "\n",
    "##### Grand canonical Ensemble\n",
    "\n",
    "$\\frac{\\partial}{\\partial \\omega_{n}}\\left\\{\\begin{array}{l}-k T r(\\rho \\ln \\rho)-\\beta[\\{\\operatorname{Tr}(\\rho H)-E\\}-\\mu\\{\\operatorname{Tr}(\\rho N)-N\\}]-\\alpha[\\operatorname{Tr}(\\rho)-1]\\end{array}\\right\\}=0 \\space$ (8)\n",
    "\n",
    "$\\operatorname{Tr}(N \\rho)=\\langle\\psi|N| \\psi\\rangle=\\sum_{n} \\omega_{n}\\left\\langle\\psi_{n}|N| \\psi_{n}\\right\\rangle \\space$  (9)\n",
    "\n",
    "Similar with Canonical Ensemble, by substituting (2),(3),(4),(9) into (8), and because of (7), we get\n",
    "\n",
    "$\\omega_n = \\frac{e^{-\\beta E_n}e^{\\beta\\mu N}}{\\sum_{e^{-\\beta E_n}e^{\\beta\\mu N}}}$\n"
   ]
  },
  {
   "cell_type": "markdown",
   "metadata": {},
   "source": [
    "#### 10.5\n",
    "\n",
    "$2 \\mathrm{HI} \\rightleftharpoons \\mathrm{H}_{2}+\\mathrm{I}_{2}$\n",
    "\n",
    "$K(T)=\\frac{\\rho_{\\mathrm{H}_{2}} \\rho_{\\mathrm{I}_{2}}}{\\rho_{\\mathrm{HI}}^{2}}=\\frac{q_{\\mathrm{H}_{2}} q_{\\mathrm{I}_{2}}}{q_{\\mathrm{HI}}^{2}}$\n",
    "\n",
    "transition: $\\frac{\\left(4 m_{\\mathbf{H}} m_{\\mathbf{I}}\\right)^{\\mathbf{3} / 2}}{\\left(m_{\\mathbf{H}}+m_{\\mathbf{I}}\\right)^{\\mathbf{3}}}$\n",
    "\n",
    "rotation: $\\theta_{r,HI}^2/(\\theta_{r,H_2}*\\theta_{r,I_2})$\n",
    "\n",
    "vibration: $e^{-2\\theta_{v,HI} / 2 T}/e^{-\\theta_{v,H_2} / 2 T}*e^{-\\theta_{v,I_2} / 2 T}$\n",
    "\n",
    "K(700K) = "
   ]
  },
  {
   "cell_type": "code",
   "execution_count": 41,
   "metadata": {},
   "outputs": [],
   "source": [
    "import numpy as np\n",
    "a = np.power(4*127,1.5)/(np.power(128,3)) * (9*9/(4*85.4*0.054))* (0.011848*0.8/(0.1027**2))"
   ]
  },
  {
   "cell_type": "code",
   "execution_count": 42,
   "metadata": {},
   "outputs": [
    {
     "name": "stdout",
     "output_type": "stream",
     "text": [
      "0.021544340376818714\n"
     ]
    }
   ],
   "source": [
    "print(a)"
   ]
  },
  {
   "cell_type": "code",
   "execution_count": 39,
   "metadata": {},
   "outputs": [],
   "source": [
    "a=np.exp(-3200/(2*700))"
   ]
  },
  {
   "cell_type": "code",
   "execution_count": 40,
   "metadata": {},
   "outputs": [
    {
     "name": "stdout",
     "output_type": "stream",
     "text": [
      "0.10170139230422684\n"
     ]
    }
   ],
   "source": [
    "print(a)"
   ]
  },
  {
   "cell_type": "markdown",
   "metadata": {},
   "source": [
    "### CAP 6610 Machine Learning\n",
    "\n",
    "#### Homework 1\n",
    "\n",
    "1.$\\space$a)$\\space$ The distribution is normalized: $\\space$ $\\int_{a}^{b} p(x;a,b) dx = \\int_{a}^{b} \\frac{1}{b-a} dx = \\frac{b-a}{b-a} = 1$\n",
    "\n",
    "$\\space$b) Mean: $\\mathrm{E}[X] =\\int_{-\\infty}^{\\infty} x p(x;a,b) d x =\\int_{a}^{b} x \\frac{1}{b-a} d x =\\frac{1}{b-a} \\int_{a}^{b} x d x =\\frac{1}{b-a}\\left[\\frac{1}{2} x^{2}\\right]_{a}^{b} =\\frac{1}{b-a} \\frac{1}{2}\\left[b^{2}-a^{2}\\right] =\\frac{(b-a)(b+a)}{2(b-a)} =\\frac{b+a}{2}$\n",
    "\n",
    "$\\space$c) Variance: $\\mathrm{E}\\left[x^{2}\\right] =\\int_{-\\infty}^{\\infty} x^{2} p(x;a,b) d x =\\int_{a}^{b} x^{2} \\frac{1}{b-a} d x =\\frac{1}{b-a} \\int_{a}^{b} x^{2} d x =\\frac{1}{b-a}\\left[\\frac{1}{3} x^{3}\\right]_{a}^{b} =\\frac{1}{b-a} \\frac{1}{3}\\left[b^{3}-a^{3}\\right] =\\frac{(b-a)\\left(b^{2}+b a+a^{2}\\right)}{3(b-a)} =\\frac{b^{2}+b a+a^{2}}{3} =\\frac{(4-3) b^{2}+(4-6) b a+(4-3) a^{2}}{12} =\\frac{b^{2}-2 b a+b^{2}}{12} =\\frac{(b-a)^{2}}{12} $\n",
    "\n",
    "2.$\\space$ a) $\\space$ By knowing that there are at least one boy, it reduces the sample space from $\\{BG,GB,BB,GG\\}$ to $\\{BG,GB,BB\\}$,so $P(one\\space child \\space is \\space girl)=\\frac{2}{3}$ \n",
    "\n",
    "$\\space$ b) $\\space$ In $\\{BG,GB,BB,GG\\}$, there is $\\frac{1}{8}$ probability that the boy who ran past was the first B of BB, and $\\frac{1}{8}$ probability he was the second boy of BB, and $\\frac{1}{8}$ probability he was the boy of BG and $\\frac{1}{8}$ probability of being the boy of GB. 4 events with equal probability, so  $P(the\\space other \\space child \\space is \\space girl)=\\frac{1}{2}$ \n",
    "\n",
    "3.$\\space$\n",
    "\n",
    "$\\begin{aligned} \\operatorname{var}(X+Y) &=E[(X+Y)(X+Y)]-E[X+Y]^{2} \\\\ &=E\\left[X^{2}+2 X Y+Y^{2}\\right]-\\left(\\mu_{x}+\\mu_{y}\\right)^{2} \\\\ &=E\\left[X^{2}+2 X Y+Y^{2}\\right]-\\mu_{x}^{2}-2 \\mu_{x} \\mu_{y}-\\mu_{y}^{2} \\\\ &=\\left(E\\left[X^{2}\\right]-\\mu_{x}^{2}\\right)+\\left(E\\left[Y^{2}\\right]-\\mu_{y}^{2}\\right)+2\\left(E[X Y]-\\mu_{x} \\mu_{y}\\right) \\\\ &=\\operatorname{var}(X)+\\operatorname{var}(Y)+2 \\operatorname{cov}(X, Y) \\end{aligned}$\n",
    "\n",
    "4.$\\space$\n",
    "\n",
    "$\\begin{aligned} & \\operatorname{cov}(X, Y) \\\\=& E\\left(\\left(X-\\mu_{X}\\right)\\left(Y-\\mu_{Y}\\right)\\right) \\\\=& E\\left(X Y-\\mu_{X} Y-X \\mu_{Y}+\\mu_{X} \\mu_{Y}\\right) \\\\=& E(X Y)-\\mu_{X} E(Y)-E(X) \\mu_{Y}+\\mu_{X} \\mu_{Y} \\\\=& E(X Y)-\\mu_{X} \\mu_{Y} \\end{aligned}$\n",
    "\n",
    "If $X$ and $Y$ are independent variables, \n",
    "\n",
    "$\\operatorname{cov}(X,Y) = E(XY) - \\mu_{X} \\mu_{Y} = E(X)E(Y) - \\mu_{X} \\mu_{Y} = 0$\n",
    "\n",
    "5.$\\space$\n",
    "\n",
    "$\\space$a) \n",
    "\n",
    "$\\begin{aligned} E(x+z) &=\\sum_{x} \\sum_{z}(x+z) P_{x z}(x, z) \\\\ &=\\sum_{x} \\sum_{z} x P_{x z}(x, z)+\\sum_{z} \\sum_{x} z P_{x z}(x, z) \\\\ &=\\sum_{x} x P_{x}(x)+z P_{z}(z) \\\\ &=E(x)+E(z) \\end{aligned}$\n",
    "\n",
    "$\\space$b) Following derivation of question 3 and 4:\n",
    "\n",
    "$\\operatorname{var}(x+z) = \\operatorname{var}(x)+\\operatorname{var}(z)+2 \\operatorname{cov}(x,z) = \\operatorname{var}(x)+\\operatorname{var}(z) $ because $x$ and $z$ are statistically independent variables.\n",
    "\n",
    "6.$\\space$for $x_{1}=0, x_{2}=n$ and $x_{1}=1, x_{2}=n-1$\n",
    "\n",
    "$\\mathcal{F}\\left(0\\right)+\\alpha \\mathcal{F}\\left(n\\right)=\\mathcal{F}\\left(\\mathcal{F}\\left(n\\right)\\right)$ $\\space$ 1)\n",
    "\n",
    "$\\mathcal{F}\\left(\\alpha\\right)+\\alpha \\mathcal{F}\\left(n-1\\right)=\\mathcal{F}\\left(\\mathcal{F}\\left(n\\right)\\right)$ 2)\n",
    "\n",
    "from 1) and 2), $\\mathcal{F}\\left(\\alpha\\right)+\\alpha \\mathcal{F}\\left(n-1\\right) = \\mathcal{F}\\left(0\\right)+\\alpha \\mathcal{F}\\left(n\\right)$\n",
    "\n",
    "so, $\\sum_{n=1}^{n}\\mathcal{F}\\left(n\\right)-\\mathcal{F}\\left(n-1\\right) = \\mathcal{F}\\left(n\\right)-\\mathcal{F}\\left(0\\right) = n\\frac{\\mathcal{F}(\\alpha) - \\mathcal{F}(0)}{\\alpha}$\n",
    "\n",
    "so, $\\mathcal{F}(n)=kn+b, $ where $ k=\\frac{\\mathcal{F}(\\alpha) - \\mathcal{F}(0)}{\\alpha}; b=\\mathcal{F}\\left(0\\right)$\n",
    "\n",
    "$\\mathcal{G}=\\underset{f \\in \\mathcal{C}}{\\operatorname{argmin}} \\sum_{i=1}^{N}\\left(y_{i}-f\\left(x_{i}\\right)\\right)^{2}$ $=$$\\mathcal{G}=\\underset{f \\in \\mathcal{C}}{\\operatorname{argmin}} \\sum_{i=1}^{N}\\left(y_{i}-kx_i -b-\\epsilon\\right)^{2}$\n",
    "\n",
    "By satisfying $\\frac{dG}{dk} = 0;$ $\\frac{dG}{db} = 0$ and $\\frac{dG}{d\\epsilon} = 0$, we get $k=\\frac{\\sum_{i=1}^{N} y_{i}\\left(x_{i}-\\bar{x}\\right)}{\\sum_{i=1}^{k} x_{i}^{2}-\\frac{1}{n}\\left(\\sum_{i=1}^{N} x_{i}\\right)^{2}}$ and $b=\\frac{\\sum_{i=1}^{N}\\left(y_{i}-\\omega x_{i}\\right)}{N}-\\varepsilon$\n",
    "\n",
    "\n",
    "\n",
    "\n",
    "\n",
    "7.$\\space$ Because there exists an uncountable family of mutually disjoint Borel subsets of  $R$. If we consider subsets $F$ of $2^R$, branches of the tree $2^R$ are disjoint and Borel.\n",
    "\n",
    "8.$\\space$  a) $\\Omega=\\left\\{\\left(x_{1}, \\cdots, x_{n}\\right): x_{i} \\in\\{H, T\\}\\right\\}$\n",
    "$F = \\{\\emptyset, \\Omega\\}$ $F $ is $\\sigma$-algebra because:\n",
    "\n",
    "1) $\\Omega \\in \\mathcal{F}$ and $\\emptyset \\in \\mathcal{F}(\\emptyset$ denotes the empty set $)$\n",
    "\n",
    "2) If $A \\in \\mathcal{F}$ then $\\Omega \\backslash A=A^{c} \\in \\mathcal{F}:$ The complementary subset of $A$ is also in $\\Omega$\n",
    "\n",
    "3) For all $A_{i} \\in \\mathcal{F}: \\bigcup_{i=1}^{\\infty} A_{i} \\in \\mathcal{F}$\n",
    "\n",
    "b) $\\space$ $F$ is countable, because $\\Omega$ is countable, which means Head can be got with finite trials.\n",
    "\n",
    "c) $P(w_i) = p_i,$ where $w_i$ is $ (x_1, x_2,...,x_i) $. \n",
    "\n",
    "\n",
    "Because:\n",
    "\n",
    "$\\mathrm{P}(\\Omega)=1$\n",
    "\n",
    "If $A \\in \\Omega$, then $P(A) \\geq 0$\n",
    "\n",
    "If $A_{1}, A_{2}, A_{3}, \\ldots \\in \\Omega$ are mutually disjoint, then $\n",
    "P\\left(\\bigcup_{i=1}^{\\infty} A_{i}\\right)=\\sum_{i=1}^{\\infty} P\\left(A_{i}\\right)$\n",
    "\n",
    "d) Because the set $F$ is countable, so $\\lim _{x \\rightarrow+\\infty} P(X \\leq x) = P(\\Omega) = 1$\n",
    "\n",
    "Probability funtion: $p_{X}(x)=(1-p)^{x} p $, where $p \\in (0,1)$ means the probability of getting head using this biased coin.\n",
    "\n",
    "$\\mathrm{E}[X]$\n",
    "$=\\sum_{x=0}^{\\infty}(1-p)^{x} p x$\n",
    "$=(1-p) p \\sum_{x=0}^{\\infty}(1-p)^{x-1} x$\n",
    "$=-(1-p) p \\sum_{x=0}^{\\infty} \\frac{d}{d p}(1-p)^{x}$\n",
    "$=-(1-p) p \\frac{d}{d p} \\sum_{x=0}^{\\infty}(1-p)^{x}$\n",
    "$=-(1-p) p \\frac{d}{d p} \\frac{1}{1-(1-p)}$\n",
    "$=-(1-p) p \\frac{d}{d p} \\frac{1}{p}$\n",
    "$=-(1-p) p\\left(-p^{-2}\\right)$\n",
    "$=\\left(p-p^{2}\\right) p^{-2}$\n",
    "$=\\frac{1}{p}-1$\n",
    "$=\\frac{1-p}{p}$\n",
    "\n",
    "\n",
    "9.$\\space$ Let $A_{n}=\\left\\{X_{n} \\leq x\\right\\}$\n",
    "\n",
    "We get \n",
    "\n",
    "$\\liminf A_{n}=\\bigcup_{n \\geq 1} \\bigcap_{k \\geq n} A_{k}$, where $\\left\\{\\cap_{k \\geq n} A_{k}\\right\\}_{n=1}^{\\infty}$ is a sequence which increase to $lim \\space inf A_n$, \n",
    "\n",
    "then $P\\left(\\liminf A_{n}\\right)=\\lim _{n \\rightarrow \\infty} P\\left(\\bigcap_{k \\geq n} A_{k}\\right)\\space$ (1) following the continuity of $P$. \n",
    "\n",
    "Since $\\forall n, \\cap_{k \\geq n} A_{k} \\subseteq A_{n}$$\\rightarrow \\forall n, P\\left(\\cap_{k \\geq n} A_{k}\\right) \\leq P\\left(A_{n}\\right)$, so $\\liminf _{n \\rightarrow \\infty} P\\left(\\bigcap_{k \\geq n} A_{k}\\right) \\leq \\liminf _{n \\rightarrow \\infty} P\\left(A_{n}\\right)\\space$ (2)\n",
    "\n",
    "Combining  above (1) and (2), we get $P\\left(\\liminf _{n \\rightarrow \\infty} A_{n}\\right) \\leq \\liminf _{n \\rightarrow \\infty} P\\left(A_{n}\\right)$."
   ]
  },
  {
   "cell_type": "code",
   "execution_count": null,
   "metadata": {},
   "outputs": [],
   "source": []
  }
 ],
 "metadata": {
  "hide_input": false,
  "kernelspec": {
   "display_name": "Python 3",
   "language": "python",
   "name": "python3"
  },
  "language_info": {
   "codemirror_mode": {
    "name": "ipython",
    "version": 3
   },
   "file_extension": ".py",
   "mimetype": "text/x-python",
   "name": "python",
   "nbconvert_exporter": "python",
   "pygments_lexer": "ipython3",
   "version": "3.6.10"
  }
 },
 "nbformat": 4,
 "nbformat_minor": 2
}
